#+TITLE: Fundamentals of Computing
** Tutorial 1 (15th October 2013)


**** 1. Brown, Jones and Smith are suspected of income tax evasion. They testify under oath as follows:


     - Brown: Jones is guilty and Smith is innocent.
     - Jones: If Brown is guilty, then so is Smith.
     - Smith: Im innocent, but at least one of the others is guilty.


**** Assuming everyones testimony is true, who is innocent and who is guilty?

***** answer:
#+begin_example
     A = Jones Guilty
     B = Smith Guilty
     C = Brown Guilty
#+end_example
     (A ∧ ¬B)
     | A B | A | ∧ | ¬B |
     |-----+---+---+----|
     | 0 0 |   | 0 |  1 |
     | 0 1 |   | 0 |  0 |
     | 1 0 |   | 1 |  1 |
     | 1 1 |   | 0 |  0 |

     (B → C)
     | B C | B | → | C |
     |-----+---+---+---|
     | 0 0 |   | 1 |   |
     | 0 1 |   | 1 |   |
     | 1 0 |   | 0 |   |
     | 1 1 |   | 1 |   |

     (¬B ∧ (A ∨ C))
     | A B C | ¬B | ∧ | (A | ∨ | C) |
     |-------+----+---+----+---+----|
     | 0 0 0 |  1 | 0 |    | 0 |    |
     | 0 0 1 |  1 | 1 |    | 1 |    |
     | 0 1 0 |  0 | 1 |    | 1 |    |
     | 1 0 0 |  1 | 0 |    | 0 |    |
     | 0 1 1 |  0 | 1 |    | 1 |    |
     | 1 1 0 |  0 | 0 |    | 1 |    |
     | 1 0 1 |  1 | 0 |    | 1 |    |
     | 1 1 1 |  0 | 0 |    | 1 |    |

     (A ∧ ¬B) ∧ (B -> C) ∧ (¬B ∧ (A ∨ C))
     | A B C | (A | ∧ | ¬B) | ∧ | (B | → | C) | ∧ | (¬B | ∧ | (A | ∨ | C)) |
     |-------+----+---+-----+---+----+---+----+---+-----+---+----+---+-----|
     | 0 0 0 |    | 0 |   1 | 0 |    | 1 |    | 0 |   1 | 0 |    | 0 |     |
     | 0 0 1 |    | 0 |   1 | 0 |    | 1 |    | 1 |   1 | 1 |    | 1 |     |
     | 0 1 0 |    | 0 |   0 | 0 |    | 0 |    | 0 |   0 | 0 |    | 0 |     |
     | 1 0 0 |    | 1 |   1 | 1 |    | 1 |    | 1 |   1 | 1 |    | 1 |     |
     | 0 1 1 |    | 0 |   0 | 0 |    | 1 |    | 1 |   0 | 1 |    | 1 |     |
     | 1 1 0 |    | 0 |   0 | 0 |    | 0 |    | 0 |   0 | 1 |    | 1 |     |
     | 1 0 1 |    | 1 |   1 | 0 |    | 1 |    | 1 |   1 | 1 |    | 1 |     |
     | 1 1 1 |    | 0 |   0 | 0 |    | 1 |    | 0 |   0 | 0 |    | 1 |     |
#+begin_example
     A = 1 true
     B = 0 false
     C = 0 false

     Jones = Guilty
     Smith = Innocent
     Brown = Innocent
#+end_example
-----

**** 2. What is the truth-value of the formula (A∧C)∨((¬B∧C) → ¬A) for A = 1, B = 1, C = 0?

     | A B C | (A | ∧ | C) | ∨ | ((¬B | ∧ | C) | → | ¬A) |
     |-------+----+---+----+---+------+---+----+---+-----|
     | 1 1 0 |    | 0 |    | 1 |    0 | 0 |    | 1 |   0 |

     0 ∨ 1 = 1
-----

**** 3. Construct the truth-table for the formula A ∨ (B ∧ C).

     | A B C | A | ∨ | (B | ∧ | C) |
     |-------+---+---+----+---+----|
     | 0 0 0 |   | 0 |    | 0 |    |
     | 0 0 1 |   | 0 |    | 0 |    |
     | 0 1 0 |   | 0 |    | 0 |    |
     | 1 0 0 |   | 1 |    | 0 |    |
     | 0 1 1 |   | 1 |    | 1 |    |
     | 1 1 0 |   | 1 |    | 0 |    |
     | 1 0 1 |   | 1 |    | 0 |    |
     | 1 1 1 |   | 1 |    | 1 |    |

-----

**** 4. Construct the truth-table for the formula A ∧ (B → C) ∧ (¬B ∨ ¬A).

     | A B C | A | ∧ | (B | → | C) | ∧ | (¬B | ∨ | ¬A) |
     |-------+---+---+----+---+----+---+-----+---+-----|
     | 0 0 0 |   | 0 |    | 1 |    | 1 |   1 | 1 |  1  |
     | 0 0 1 |   | 0 |    | 1 |    | 1 |   1 | 1 |  1  |
     | 0 1 0 |   | 0 |    | 0 |    | 0 |   0 | 1 |  1  |
     | 1 0 0 |   | 1 |    | 1 |    | 1 |   1 | 1 |  0  |
     | 0 1 1 |   | 0 |    | 1 |    | 0 |   0 | 1 |  1  |
     | 1 1 0 |   | 1 |    | 1 |    | 0 |   0 | 0 |  0  |
     | 1 0 1 |   | 0 |    | 0 |    | 0 |   1 | 1 |  0  |
     | 1 1 1 |   | 1 |    | 1 |    | 0 |   0 | 0 |  0  |

-----

**** 5. Determine whether the formulas A ∧ (B ⊕ C) and (A ∧ B) ⊕ (A ∧ C) are equivalent, where ⊕ denotes ‘exclusive OR’ (or ‘XOR’).

     A ∧ (B ⊕ C)
     | A B C | A | ∧ | (B | ⊕ | C) |
     |-------+---+---+----+---+----|
     | 0 0 0 |   | 0 |    | 0 |    |
     | 0 0 1 |   | 0 |    | 1 |    |
     | 0 1 0 |   | 0 |    | 1 |    |
     | 1 0 0 |   | 0 |    | 0 |    |
     | 0 1 1 |   | 0 |    | 0 |    |
     | 1 1 0 |   | 1 |    | 1 |    |
     | 1 0 1 |   | 1 |    | 1 |    |
     | 1 1 1 |   | 0 |    | 0 |    |

     (A ∧ B) ⊕ (A ∧ C)
     | A B C | (A | ∧ | B) | ⊕ | (A | ∧ | C) |
     |-------+----+---+----+---+----+---+----|
     | 0 0 0 |    | 0 |    | 0 |    | 0 |    |
     | 0 0 1 |    | 0 |    | 0 |    | 0 |    |
     | 0 1 0 |    | 0 |    | 0 |    | 0 |    |
     | 1 0 0 |    | 0 |    | 0 |    | 0 |    |
     | 0 1 1 |    | 0 |    | 0 |    | 0 |    |
     | 1 1 0 |    | 1 |    | 1 |    | 0 |    |
     | 1 0 1 |    | 0 |    | 1 |    | 1 |    |
     | 1 1 1 |    | 1 |    | 0 |    | 1 |    |

     Yes they are equivalent.

-----

**** 6. Construct a Boolean formula that realises the Boolean function given by the following truth-table:

     | x1 x2 x3 | f(x1, x2, x3) |                                       |
     |----------+---------------+---------------------------------------|
     | 0  0  0  |             0 |                                       |
     | 0  0  1  |             0 |                                       |
     | 0  1  0  |             1 | (a) use the connectives ∨, ∧, ¬ only; |
     | 0  1  1  |             1 | (b) find a shortest possible formula. |
     | 1  0  0  |             0 |                                       |
     | 1  0  1  |             1 |                                       |
     | 1  1  0  |             0 |                                       |
     | 1  1  1  |             1 |                                       |

***** answer:

#+begin_example

   0    1     0       0    1    1      1     0    1      1    1    1
(¬x1 ∧ x2 ∧ ¬x3) ∨ (¬x1 ∧ x2 ∧ x3) ∨ (x1 ∧ ¬x2 ∧ x3) ∨ (x1 ∧ x2 ∧ x3)
A = ¬x1 ∧ x2
B = x1 ∧ x3

(A ∧ ¬x3) ∨ (A ∧ x3) ∨ (B ∧ ¬x2) ∨ (B ∧ x2)
B ∧ 1 = B ∧ (x2 ∨ ¬x2)
B

(A ∧ ¬x3) ∨ (A ∧ x3)
A ∧ 1 = A ∧ (x3 ∨ ¬x3)
A

A ∨ B = (¬x1 ∧ x2) ∨ (x1 ∧ x3)

#+end_example

-----

**** 7. Consider the Boolean function f(x1, x2, x3) realised by the following Boolean circuit:

    ￼x1 ∧ (x2 ∨ ¬x3)
***** answer:

    | x1 x2 x3 | x1 | ∧ | (x2 | ∨ | ¬x3)  |
    |----------+----+---+-----+---+------|
    | 0  0  0  |    | 0 |     | 1 |      |
    | 0  0  1  |    | 0 |     | 0 |      |
    | 0  1  0  |    | 0 |     | 1 |      |
    | 1  0  0  |    | 1 |     | 1 |      |
    | 0  1  1  |    | 0 |     | 1 |      |
    | 1  1  0  |    | 1 |     | 1 |      |
    | 1  0  1  |    | 0 |     | 0 |      |
    | 1  1  1  |    | 1 |     | 1 |      |

-----

**** 8. A 2-to-1 multiplexer has three inputs, say A0, A1 and S; the output is A0 if S = 0 and A1 if S = 1. Design a Boolean circuit for the 2-to-1 multiplexer.

***** answer:

     | A0 A1 S | f(A0 A1 S) |
     |---------+------------|
     | 0  0  0 |      0     |
     | 0  0  1 |      0     |
     | 0  1  0 |      0     |
     | 1  0  0 |      1     |
     | 0  1  1 |      1     |
     | 1  1  0 |      1     |
     | 1  0  1 |      0     |
     | 1  1  1 |      1     |

#+begin_example
      1     0     0      0    1    1     1    1     0     1    1    1
     (A0 ∧ ¬A1 ∧ ¬S) ∨ (¬A0 ∧ A1 ∧ S) ∨ (A0 ∧ A1 ∧ ¬S) ∨ (A0 ∧ A1 ∧ S)

     B = A0 ∧ A1
     (A0 ∧ ¬A1 ∧ ¬S) ∨ (¬A0 ∧ A1 ∧ S) ∨ (B ∧ ¬S) ∨ (B ∧ S)
     B ∧ (S ∨ ¬S) = (B ∧ ¬S) ∨ (B ∧ S)
     B ∧ 1
     B

     (A0 ∧ ¬A1 ∧ ¬S) ∨ (¬A0 ∧ A1 ∧ S) ∨ B
     (A0 ⊕ (A1 ∧ S)) ∨ B

     (A0 ⊕ (A1 ∧ S)) ∨ (A0 ∧ A1)
#+end_example
-----

**** 9. Let f(x0,x1,x2) be the Boolean function checking whether a given 3-bit binary number (x2x1x0) is divisible by 3. More precisely, f(x0,x1,x2) = 1 if and only if the number (x2x1x0)2 is divisible by 3.
